CPL_Completeness.thy
@@ -73,7 +73,6 @@ termination canonicalJudgementRec
   apply (auto)
   done
 
-
 fun canonicalJudgement :: "nat \<Rightarrow> Formula \<Rightarrow> 'a Structure \<Rightarrow> 'a Judgement" where
 "canonicalJudgement 0 \<phi> \<B> = (Judgement 0 {} {})" |
 "canonicalJudgement i \<phi> \<B> = (let
@@ -82,7 +81,7 @@ fun canonicalJudgement :: "nat \<Rightarrow> Formula \<Rightarrow> 'a Structure 
     (if ((i = 0) \<or> (i > (length \<phi>\<^sub>L)) \<or> ((length \<phi>\<^sub>L) = 0))
       then (Judgement 0 {} {})
       else (canonicalJudgementRec (FoI i \<phi>\<^sub>L) i \<phi>\<^sub>L P\<^sub>L \<B>)
-    )
+    )                      
   )
 )"
 
@@ -104,6 +103,7 @@ proof -
 qed
 *)
 
+(*
 lemma canonical_judgement_lemma_index [simp] :
   fixes \<phi> :: Formula
   fixes \<B> :: "'a Structure"
@@ -111,37 +111,68 @@ lemma canonical_judgement_lemma_index [simp] :
   fixes \<J>\<^sub>c :: "'a Judgement"
   assumes "(wfCPLInstance \<phi> \<B>)"
   assumes "(i \<in> (setOfIndex (formulaToList \<phi>)))"
-  shows "(Index (canonicalJudgement i \<phi> \<B>)) = i"
+  assumes "\<J>\<^sub>c = (canonicalJudgement i \<phi> \<B>)"
+  shows "(Index \<J>\<^sub>c) = i"
 proof -
   let ?formulaParentList = "buildFormulaParentList \<phi>"
   obtain \<J>\<^sub>c where "\<J>\<^sub>c = (canonicalJudgement i \<phi> \<B>)" by simp
   obtain \<phi>\<^sub>L where "\<phi>\<^sub>L = fst ?formulaParentList" by simp
   obtain P\<^sub>L where "P\<^sub>L = snd ?formulaParentList" by simp
   obtain \<psi> where "\<psi> = (FoI i \<phi>\<^sub>L)" by simp
-  have "(Index \<J>\<^sub>c) = i"
-  show ?thesis 
+  show ?thesis sorry
 qed
+*)
 
+(*
+lemma canonical_judgement_lemma_var_set [simp] :
+  fixes \<phi> :: Formula
+  fixes \<B> :: "'a Structure"
+  fixes i :: nat
+  fixes \<J>\<^sub>c :: "'a Judgement"
+  fixes \<phi>\<^sub>L :: "Formula list"
+  assumes "(wfCPLInstance \<phi> \<B>)"
+  assumes "(i \<in> (setOfIndex (formulaToList \<phi>)))"
+  assumes "\<J>\<^sub>c = (canonicalJudgement i \<phi> \<B>)"
+  assumes "\<phi>\<^sub>L = (fst (buildFormulaParentList \<phi>))"
+  shows "(Vars \<J>\<^sub>c) = (freeVar (FoI i \<phi>\<^sub>L))"
+proof -
+  let ?formulaParentList = "buildFormulaParentList \<phi>"
+  obtain \<J>\<^sub>c where "\<J>\<^sub>c = (canonicalJudgement i \<phi> \<B>)" by simp
+  obtain \<phi>\<^sub>L where "\<phi>\<^sub>L = fst ?formulaParentList" by simp
+  obtain P\<^sub>L where "P\<^sub>L = snd ?formulaParentList" by simp
+  obtain \<psi> where "\<psi> = (FoI i \<phi>\<^sub>L)" by simp
+  show ?thesis sorry
+qed
+*)
+
+lemma canonical_judgement_is_always_well_formed [simp] : "\<lbrakk>
+  (wfCPLInstance \<phi> \<B>);
+  (i \<in> (setOfIndex (snd (buildFormulaParentList \<phi>))))
+\<rbrakk> \<Longrightarrow> (wfJudgement (canonicalJudgement i \<phi> \<B>)) \<phi> \<B>"
+  apply (auto)
+  apply (simp_all add: Let_def)
+  sorry
 
 
 lemma canonical_judgement_lemma_is_derivable [simp] :
   fixes \<phi> :: Formula
   fixes \<B> :: "'a Structure"
   fixes i :: nat
-  fixes \<J>\<^sub>c :: "'a Judgement"
   assumes "(wfCPLInstance \<phi> \<B>)"
-  assumes "(i \<in> (setOfIndex (formulaToList \<phi>)))"
-  assumes "\<J>\<^sub>c = (canonicalJudgement i \<phi> \<B>)"
-  shows "isDerivable \<phi> \<B> \<J>\<^sub>c"
+  assumes "(i \<in> (setOfIndex (snd (buildFormulaParentList \<phi>))))"
+  shows "isDerivable \<phi> \<B> (canonicalJudgement i \<phi> \<B>)"
 proof -        
   let ?formulaParentList = "buildFormulaParentList \<phi>"
+  obtain \<J>\<^sub>c where canonical_judgement: "\<J>\<^sub>c = (canonicalJudgement i \<phi> \<B>)" by simp
   obtain \<phi>\<^sub>L where "\<phi>\<^sub>L = fst ?formulaParentList" by simp
   obtain P\<^sub>L where "P\<^sub>L = snd ?formulaParentList" by simp
   obtain \<psi> where "\<psi> = (FoI i \<phi>\<^sub>L)" by simp
-  show ?thesis
-  proof (cases \<psi>)
-  case (Atom r var_list)
-    then show ?thesis
+  show ?thesis sorry
+  (*proof (cases \<psi>)
+    case (Atom r var_list)
+    have wf_judgement: "wfJudgement \<J>\<^sub>c \<phi> \<B>" sorry
+    have "isAtom \<J>\<^sub>c \<phi> \<B>" sorry
+    thus ?thesis using ATR wf_judgement assms(1) canonical_judgement by blast
   next
     case (And \<psi>\<^sub>1 \<psi>\<^sub>2)
     then show ?thesis sorry
@@ -151,7 +182,7 @@ proof -
   next
     case (Exists x \<psi>\<^sub>1)
     then show ?thesis sorry
-  qed
+  qed*)
 qed
 
 
@@ -165,13 +196,69 @@ theorem CPL_Completeness_Theorem [simp] :
   assumes "\<not>(isModel \<B> e \<phi>)"
   shows "isDerivable \<phi> \<B> (Judgement 1 {} {})"
 proof -
-  show ?thesis by sorry
+  have "(wfStructure \<B>)" using assms(1) by auto 
+  have "(wfFormula \<phi> (Sig \<B>))" using assms(1) by auto 
+  have "((ran e) \<subseteq> (Univ \<B>))" by simp
+  have "sentence \<phi>" using assms(1) by auto
+  let ?formulaParentList = "buildFormulaParentList \<phi>"
+  obtain P\<^sub>L where "P\<^sub>L = snd ?formulaParentList" by simp
+  have "(1 \<in> (setOfIndex P\<^sub>L))" using \<open>P\<^sub>L = snd (buildFormulaParentList \<phi>)\<close> one_is_always_in_set_of_index prod.collapse by blast
+  show ?thesis
+  proof (cases \<phi>)
+    case (Atom r var_list)
+    have "(set var_list) = (freeVar \<phi>)" by (simp add: Atom)
+    have "((freeVar \<phi>) \<subseteq> (dom e))" using \<open>sentence \<phi>\<close> by auto
+    then show ?thesis
+    proof (cases "((Sig \<B>) r)")
+      case None
+      show ?thesis
+      proof (rule ccontr)
+        show "False" using Atom None \<open>wfFormula \<phi> (Sig \<B>)\<close> by auto
+      qed
+    next
+      case (Some arity)
+      show ?thesis
+      proof (cases "arity = 0")
+        case False
+        have "arity > 0" using False by auto
+        have "(isFormulaAtom \<phi>)" by (simp add: Atom) 
+        have "((length var_list) = arity)" using Atom Some \<open>wfFormula \<phi> (Sig \<B>)\<close> by force
+        show ?thesis
+        proof (rule ccontr)
+          have "\<not> (sentence \<phi>)" using Atom \<open>0 < arity\<close> \<open>length var_list = arity\<close> by auto
+          thus "False" using \<open>sentence \<phi>\<close> by blast 
+        qed
+      next
+        case True \<comment> \<open>He supuesto que aceptamos símbolos de relacion de aridad 0\<close>
+        have "(length var_list) = 0" using \<open>sentence \<phi>\<close> \<open>set var_list = freeVar \<phi>\<close> by auto
+        obtain \<J>\<^sub>c where "\<J>\<^sub>c = canonicalJudgement 1 \<phi> \<B>" by auto
+        have "isDerivable \<phi> \<B> \<J>\<^sub>c" using \<open>1 \<in> setOfIndex P\<^sub>L\<close> \<open>P\<^sub>L = snd (buildFormulaParentList \<phi>)\<close> \<open>\<J>\<^sub>c = canonicalJudgement 1 \<phi> \<B>\<close> assms(1) canonical_judgement_lemma_is_derivable by blast
+        have "\<J>\<^sub>c = (Judgement 1 {} {})" sorry
+        show ?thesis using \<open>\<J>\<^sub>c = NullJudgement\<close> \<open>isDerivable \<phi> \<B> \<J>\<^sub>c\<close> by blast
+      qed
+    qed
+  next
+    case (And \<psi>\<^sub>1 \<psi>\<^sub>2)
+    obtain \<J>\<^sub>c where "\<J>\<^sub>c = canonicalJudgement 1 \<phi> \<B>" by auto
+    have "isDerivable \<phi> \<B> \<J>\<^sub>c" sorry
+    then show ?thesis sorry
+  next
+    case (Forall x \<psi>)
+    obtain \<J>\<^sub>c where "\<J>\<^sub>c = canonicalJudgement 1 \<phi> \<B>" by auto
+    have "isDerivable \<phi> \<B> \<J>\<^sub>c" sorry
+    then show ?thesis sorry
+  next
+    case (Exists x \<psi>)
+    obtain \<J>\<^sub>c where "\<J>\<^sub>c = canonicalJudgement 1 \<phi> \<B>" by auto
+    have "isDerivable \<phi> \<B> \<J>\<^sub>c" sorry
+    then show ?thesis sorry
+  qed
 qed
+
 
 (* ==================== Tests ==================== *)
 
 lemma "(canonicalJudgement 10 myFormula myStructure) = (Judgement 0 {} {})"
-  apply (auto)
   apply (simp add: numeral_nat(2) numeral_Bit1)
   done
 
